---
title: Matrix cookbook - Derivative
date: 2019-10-24
tags: [Matrix, derivative]
---

\begin{equation}
\tag{40}
\partial\left(\mathbf{X}^{-1}\right)=-\mathbf{X}^{-1}(\partial \mathbf{X}) \mathbf{X}^{-1}
\end{equation}

Explanation: [^1]
\begin{equation}
\underbrace{(I)^{\prime}}_{=0}=\left(\mathbf{X} \mathbf{X}^{-1}\right)^{\prime}=\mathbf{X}^{\prime} \mathbf{X}^{-1}+\mathbf{X}\left(\mathbf{X}^{-1}\right)^{\prime} \Rightarrow
\end{equation}

\begin{equation}
\mathbf{X}\left(\mathbf{X}^{-1}\right)^{\prime}=-\mathbf{X}^{\prime} \mathbf{X}^{-1} \quad \Rightarrow
\end{equation}

\begin{equation}
\left(\mathbf{X}^{-1}\right)^{\prime}=-\mathbf{X}^{-1} \mathbf{X}^{\prime} \mathbf{X}^{-1}
\end{equation}

[^1]: https://math.stackexchange.com/questions/1471825/derivative-of-the-inverse-of-a-matrix
