---
title: Matrix cookbook - Basics
date: 2019-10-10
tags: [matrix, cookbook]
header-includes:
- \usepackage{amsmath}
---

\begin{equation}
\tag{1}
(\mathbf{A B})^{-1}=\mathbf{B}^{-1} \mathbf{A}^{-1}
\end{equation}

\begin{equation}
\tag{2}
(\mathbf{A B C} \ldots)^{-1}=\ldots \mathbf{C}^{-1} \mathbf{B}^{-1} \mathbf{A}^{-1}
\end{equation}

\begin{equation}
\tag{3}
\left(\mathbf{A}^{T}\right)^{-1}=\left(\mathbf{A}^{-1}\right)^{T}
\end{equation}

\begin{equation}
\tag{4}
(\mathbf{A}+\mathbf{B})^{T}=\mathbf{A}^{T}+\mathbf{B}^{T}
\end{equation}

\begin{equation}
\tag{5}
(\mathbf{A B})^{T}=\mathbf{B}^{T} \mathbf{A}^{T}
\end{equation}

\begin{equation}
\tag{6}
(\mathbf{A B C} \ldots)^{T}=\ldots \mathbf{C}^{T} \mathbf{B}^{T} \mathbf{A}^{T}
\end{equation}
